Abstracted 'tag_const' with type classes over linordered rings (issue #8)

src/Coinductive_Prop.thy
@@ -9,7 +9,7 @@ section \<open>Stepwise denotational interpretation of TESL atoms\<close>
 
 (* Denotational interpretation of TESL bounded by index *)
 fun TESL_interpretation_atomic_stepwise
-    :: "TESL_atomic \<Rightarrow> nat \<Rightarrow> run set" ("\<lbrakk> _ \<rbrakk>\<^sub>T\<^sub>E\<^sub>S\<^sub>L\<^bsup>\<ge> _\<^esup>") where
+    :: "('\<tau>::linordered_field) TESL_atomic \<Rightarrow> nat \<Rightarrow> '\<tau> run set" ("\<lbrakk> _ \<rbrakk>\<^sub>T\<^sub>E\<^sub>S\<^sub>L\<^bsup>\<ge> _\<^esup>") where
     "\<lbrakk> K sporadic \<tau> \<rbrakk>\<^sub>T\<^sub>E\<^sub>S\<^sub>L\<^bsup>\<ge> i\<^esup> =
         { \<rho>. \<exists>n\<ge>i. hamlet ((Rep_run \<rho>) n K) = True \<and> time ((Rep_run \<rho>) n K) = \<tau> }"
   | "\<lbrakk> K\<^sub>1 sporadic \<lfloor>\<tau>\<rfloor> on K\<^sub>2 \<rbrakk>\<^sub>T\<^sub>E\<^sub>S\<^sub>L\<^bsup>\<ge> i\<^esup> =
@@ -70,18 +70,18 @@ lemma TESL_interp_unfold_stepwise_timedelayed:
 
 theorem TESL_interp_unfold_stepwise_positive_atoms:
   assumes "positive_atom \<phi>"
-  shows "\<lbrakk> \<phi> \<rbrakk>\<^sub>T\<^sub>E\<^sub>S\<^sub>L = \<Union> {Y. \<exists>n::nat. Y = \<lbrakk> \<phi> \<rbrakk>\<^sub>T\<^sub>E\<^sub>S\<^sub>L\<^bsup>\<ge> n\<^esup>}"
+  shows "\<lbrakk> \<phi>::'\<tau>::linordered_field TESL_atomic \<rbrakk>\<^sub>T\<^sub>E\<^sub>S\<^sub>L = \<Union> {Y. \<exists>n::nat. Y = \<lbrakk> \<phi> \<rbrakk>\<^sub>T\<^sub>E\<^sub>S\<^sub>L\<^bsup>\<ge> n\<^esup>}"
   proof -
-    obtain cc :: "TESL_atomic \<Rightarrow> clock" and tt :: "TESL_atomic \<Rightarrow> tag_const" and cca :: "TESL_atomic \<Rightarrow> clock" and tta :: "TESL_atomic \<Rightarrow> tag_expr" and ccb :: "TESL_atomic \<Rightarrow> clock" where
-      f1: "\<forall>t. \<not> positive_atom t \<or> t = cc t sporadic tt t \<or> t = cca t sporadic tta t on ccb t"
-      using positive_atom.elims(2) by moura
-    obtain ttb :: "tag_expr \<Rightarrow> tag_const" where
-      "\<And>c t ca. \<Union>{R. \<exists>n. R = \<lbrakk> c sporadic t on ca \<rbrakk>\<^sub>T\<^sub>E\<^sub>S\<^sub>L\<^bsup>\<ge> n\<^esup>} = \<lbrakk> c sporadic t on ca \<rbrakk>\<^sub>T\<^sub>E\<^sub>S\<^sub>L \<or> \<lfloor> ttb t \<rfloor> = t"
-      by (metis TESL_interp_unfold_stepwise_sporadicon_add old.prod.exhaust tag_expr.exhaust tag_var.exhaust)
-    then have "\<And>t. \<Union>{R. \<exists>n. R = \<lbrakk> t \<rbrakk>\<^sub>T\<^sub>E\<^sub>S\<^sub>L\<^bsup>\<ge> n\<^esup>} = \<lbrakk> t \<rbrakk>\<^sub>T\<^sub>E\<^sub>S\<^sub>L \<or> \<lfloor> ttb (tta t) \<rfloor> = tta t \<or> \<not> positive_atom t"
-      using f1 by (metis TESL_interp_unfold_stepwise_sporadic)
+    obtain cc :: "'\<tau> TESL_atomic \<Rightarrow> clock" and tt :: "'\<tau> TESL_atomic \<Rightarrow> '\<tau> tag_const" and cca :: "'\<tau> TESL_atomic \<Rightarrow> clock" and tta :: "'\<tau> TESL_atomic \<Rightarrow> '\<tau> tag_expr" and ccb :: "'\<tau> TESL_atomic \<Rightarrow> clock" where
+      f1: "cca \<phi> sporadic tta \<phi> on ccb \<phi> = \<phi> \<or> cc \<phi> sporadic tt \<phi> = \<phi>"
+      by (metis (no_types) assms positive_atom.elims(2))
+    { assume "\<Union>{R. \<exists>n. R = \<lbrakk> \<phi> \<rbrakk>\<^sub>T\<^sub>E\<^sub>S\<^sub>L\<^bsup>\<ge> n\<^esup>} \<noteq> \<lbrakk> \<phi> \<rbrakk>\<^sub>T\<^sub>E\<^sub>S\<^sub>L"
+      then have "cc \<phi> sporadic tt \<phi> \<noteq> \<phi>"
+        by (metis TESL_interp_unfold_stepwise_sporadic)
+      then have ?thesis
+        using f1 by (metis (no_types) TESL_interp_unfold_stepwise_sporadicon TESL_interp_unfold_stepwise_sporadicon_add old.prod.exhaust tag_expr.exhaust tag_var.exhaust) }
     then show ?thesis
-      using f1 by (metis TESL_interp_unfold_stepwise_sporadic TESL_interp_unfold_stepwise_sporadicon assms)
+      by blast
   qed
 
 theorem TESL_interp_unfold_stepwise_negative_atoms:
@@ -217,7 +217,7 @@ lemma TESL_interp_stepwise_timedelayed_coind_unfold:
     then show ?thesis by auto
   qed
 
-fun TESL_interpretation_stepwise :: "TESL_formula \<Rightarrow> nat \<Rightarrow> run set" ("\<lbrakk>\<lbrakk> _ \<rbrakk>\<rbrakk>\<^sub>T\<^sub>E\<^sub>S\<^sub>L\<^bsup>\<ge> _\<^esup>") where
+fun TESL_interpretation_stepwise :: "'\<tau>::linordered_field TESL_formula \<Rightarrow> nat \<Rightarrow> '\<tau> run set" ("\<lbrakk>\<lbrakk> _ \<rbrakk>\<rbrakk>\<^sub>T\<^sub>E\<^sub>S\<^sub>L\<^bsup>\<ge> _\<^esup>") where
     "\<lbrakk>\<lbrakk> [] \<rbrakk>\<rbrakk>\<^sub>T\<^sub>E\<^sub>S\<^sub>L\<^bsup>\<ge> n\<^esup> = { _. True }"
   | "\<lbrakk>\<lbrakk> \<phi> # \<Phi> \<rbrakk>\<rbrakk>\<^sub>T\<^sub>E\<^sub>S\<^sub>L\<^bsup>\<ge> n\<^esup> = \<lbrakk> \<phi> \<rbrakk>\<^sub>T\<^sub>E\<^sub>S\<^sub>L\<^bsup>\<ge> n\<^esup> \<inter> \<lbrakk>\<lbrakk> \<Phi> \<rbrakk>\<rbrakk>\<^sub>T\<^sub>E\<^sub>S\<^sub>L\<^bsup>\<ge> n\<^esup>"
 
@@ -295,13 +295,14 @@ theorem TESL_interp_stepwise_composition:
 
 section \<open>Interpretation of configurations\<close>
 
-fun HeronConf_interpretation :: "config \<Rightarrow> run set" ("\<lbrakk> _ \<rbrakk>\<^sub>c\<^sub>o\<^sub>n\<^sub>f\<^sub>i\<^sub>g" 71) where
+fun HeronConf_interpretation :: "'\<tau>::linordered_field config \<Rightarrow> '\<tau> run set" ("\<lbrakk> _ \<rbrakk>\<^sub>c\<^sub>o\<^sub>n\<^sub>f\<^sub>i\<^sub>g" 71) where
   "\<lbrakk> \<Gamma>, n \<turnstile> \<Psi> \<triangleright> \<Phi> \<rbrakk>\<^sub>c\<^sub>o\<^sub>n\<^sub>f\<^sub>i\<^sub>g = \<lbrakk>\<lbrakk> \<Gamma> \<rbrakk>\<rbrakk>\<^sub>p\<^sub>r\<^sub>i\<^sub>m \<inter> \<lbrakk>\<lbrakk> \<Psi> \<rbrakk>\<rbrakk>\<^sub>T\<^sub>E\<^sub>S\<^sub>L\<^bsup>\<ge> n\<^esup> \<inter> \<lbrakk>\<lbrakk> \<Phi> \<rbrakk>\<rbrakk>\<^sub>T\<^sub>E\<^sub>S\<^sub>L\<^bsup>\<ge> Suc n\<^esup>"
 
 lemma HeronConf_interp_composition:
   shows "\<lbrakk> \<Gamma>\<^sub>1, n \<turnstile> \<Psi>\<^sub>1 \<triangleright> \<Phi>\<^sub>1 \<rbrakk>\<^sub>c\<^sub>o\<^sub>n\<^sub>f\<^sub>i\<^sub>g \<inter> \<lbrakk> \<Gamma>\<^sub>2, n \<turnstile> \<Psi>\<^sub>2 \<triangleright> \<Phi>\<^sub>2 \<rbrakk>\<^sub>c\<^sub>o\<^sub>n\<^sub>f\<^sub>i\<^sub>g
          = \<lbrakk> \<Gamma>\<^sub>1 @ \<Gamma>\<^sub>2, n \<turnstile> \<Psi>\<^sub>1 @ \<Psi>\<^sub>2 \<triangleright> \<Phi>\<^sub>1 @ \<Phi>\<^sub>2 \<rbrakk>\<^sub>c\<^sub>o\<^sub>n\<^sub>f\<^sub>i\<^sub>g"
-  using TESL_interp_stepwise_composition symrun_interp_expansion by auto
+  using TESL_interp_stepwise_composition symrun_interp_expansion
+  by (simp add: TESL_interp_stepwise_composition symrun_interp_expansion inf_assoc inf_left_commute)
 
 lemma HeronConf_interp_stepwise_instant_cases:
   shows "\<lbrakk> \<Gamma>, n \<turnstile> [] \<triangleright> \<Phi> \<rbrakk>\<^sub>c\<^sub>o\<^sub>n\<^sub>f\<^sub>i\<^sub>g
