src/TESL.thy
@@ -10,45 +10,45 @@ type_synonym instant_index = "nat"
 
 (** Tags **) 
 (* Constants *)
-datatype tag_const =
-    Real   "real"                   ("\<tau>\<^sub>r\<^sub>a\<^sub>t")
+datatype '\<tau> tag_const =
+    Real   '\<tau>                   ("\<tau>\<^sub>r\<^sub>a\<^sub>t")
 (* Variables *)
 datatype tag_var =
     Schematic "clock * instant_index" ("\<tau>\<^sub>v\<^sub>a\<^sub>r")
 (* Expressions *)
-datatype tag_expr =
-    Const    "tag_const"           ("\<lfloor> _ \<rfloor>")
-  | AddDelay "tag_var" "tag_const" ("\<lfloor> _ \<oplus> _ \<rfloor>")
+datatype '\<tau> tag_expr =
+    Const    "'\<tau> tag_const"           ("\<lfloor> _ \<rfloor>")
+  | AddDelay "tag_var" "'\<tau> tag_const" ("\<lfloor> _ \<oplus> _ \<rfloor>")
 
 (* Primitives for symbolic runs *)
-datatype constr =
-    Timestamp "clock"   "instant_index" "tag_expr"            ("_ \<Down> _ @ _")
+datatype '\<tau> constr =
+    Timestamp "clock"   "instant_index" "'\<tau> tag_expr"            ("_ \<Down> _ @ _")
   | Ticks     "clock"   "instant_index"                       ("_ \<Up> _")
   | NotTicks  "clock"   "instant_index"                       ("_ \<not>\<Up> _")
-  | Affine    "tag_var" "tag_const"     "tag_var" "tag_const" ("_ \<doteq> _ * _ + _")
-  | ArithGen  "tag_var" "tag_var" "(tag_const \<times> tag_const) \<Rightarrow> bool" ("\<langle>_, _\<rangle> \<epsilon> _")
+  | Affine    "tag_var" "'\<tau> tag_const"     "tag_var" "'\<tau> tag_const" ("_ \<doteq> _ * _ + _")
+  | ArithGen  "tag_var" "tag_var" "('\<tau> tag_const \<times> '\<tau> tag_const) \<Rightarrow> bool" ("\<langle>_, _\<rangle> \<epsilon> _")
 
-type_synonym system = "constr list"
+type_synonym '\<tau> system = "'\<tau> constr list"
 
 text{* Define as follows the syntax of TESL *}
 
 (* TESL language *)
-datatype TESL_atomic =
-    Sporadic       "clock" "tag_const"                     (infixr "sporadic" 55)
-  | SporadicOn     "clock" "tag_expr"  "clock"             ("_ sporadic _ on _" 55)
-  | TagRelation    "clock" "tag_const" "clock" "tag_const" ("tag-relation _ = _ * _ + _" 55)
-  | TagRelationGen "clock" "clock" "(tag_const \<times> tag_const) \<Rightarrow> bool" ("tag-relation \<langle>_, _\<rangle> \<in> _" 55)
+datatype '\<tau> TESL_atomic =
+    Sporadic       "clock" "'\<tau> tag_const"                     (infixr "sporadic" 55)
+  | SporadicOn     "clock" "'\<tau> tag_expr"  "clock"             ("_ sporadic _ on _" 55)
+  | TagRelation    "clock" "'\<tau> tag_const" "clock" "'\<tau> tag_const" ("tag-relation _ = _ * _ + _" 55)
+  | TagRelationGen "clock" "clock" "('\<tau> tag_const \<times> '\<tau> tag_const) \<Rightarrow> bool" ("tag-relation \<langle>_, _\<rangle> \<in> _" 55)
   | Implies        "clock" "clock"                         (infixr "implies" 55)
-  | TimeDelayedBy  "clock" "tag_const" "clock" "clock"     ("_ time-delayed by _ on _ implies _" 55)
+  | TimeDelayedBy  "clock" "'\<tau> tag_const" "clock" "clock"     ("_ time-delayed by _ on _ implies _" 55)
 
-type_synonym TESL_formula = "TESL_atomic list"
+type_synonym '\<tau> TESL_formula = "'\<tau> TESL_atomic list"
 
-fun positive_atom :: "TESL_atomic \<Rightarrow> bool" where
+fun positive_atom :: "'\<tau> TESL_atomic \<Rightarrow> bool" where
     "positive_atom (_ sporadic _)      = True"
   | "positive_atom (_ sporadic _ on _) = True"
   | "positive_atom _                   = False"
 
-abbreviation NoSporadic :: "TESL_formula \<Rightarrow> TESL_formula" where 
+abbreviation NoSporadic :: "'\<tau> TESL_formula \<Rightarrow> '\<tau> TESL_formula" where 
   "NoSporadic f \<equiv> (List.filter (\<lambda>f\<^sub>a\<^sub>t\<^sub>o\<^sub>m. case f\<^sub>a\<^sub>t\<^sub>o\<^sub>m of
       _ sporadic _  \<Rightarrow> False
     | _ sporadic _ on _ \<Rightarrow> False
@@ -58,67 +58,67 @@ abbreviation NoSporadic :: "TESL_formula \<Rightarrow> TESL_formula" where
    Follows the intuition: past [\<Gamma>], current index [n], present [\<psi>], future [\<phi>]
    Beware: This type is slightly different from which originally implemented in Heron
 *)
-type_synonym config = "system * instant_index * TESL_formula * TESL_formula"
+type_synonym '\<tau> config = "'\<tau> system * instant_index * '\<tau> TESL_formula * '\<tau> TESL_formula"
 
 (*declare[[show_sorts]]*)
 
 (* Instanciating tag_const to give field structure *)
-instantiation tag_const :: plus
+instantiation tag_const :: (plus)plus
 begin
-  fun plus_tag_const :: "tag_const \<Rightarrow> tag_const \<Rightarrow> tag_const" where
+  fun plus_tag_const :: "'a tag_const \<Rightarrow> 'a tag_const \<Rightarrow> 'a tag_const" where
       Real_plus: "(Real n) + (Real p) = (Real (n + p))"
   instance proof qed
 end
 
-instantiation tag_const :: minus
+instantiation tag_const :: (minus)minus
 begin
-  fun minus_tag_const :: "tag_const \<Rightarrow> tag_const \<Rightarrow> tag_const" where
+  fun minus_tag_const :: "'a tag_const \<Rightarrow> 'a tag_const \<Rightarrow> 'a tag_const" where
       Real_minus: "(Real n) - (Real p) = (Real (n - p))"
   instance proof qed
 end
 
-instantiation tag_const :: times
+instantiation tag_const :: (times)times
 begin
-  fun times_tag_const :: "tag_const \<Rightarrow> tag_const \<Rightarrow> tag_const" where
+  fun times_tag_const :: "'a tag_const \<Rightarrow> 'a tag_const \<Rightarrow> 'a tag_const" where
       Real_times: "(Real n) * (Real p) = (Real (n * p))"
   instance proof qed
 end
 
-instantiation tag_const :: divide
+instantiation tag_const :: (divide)divide
 begin
-  fun divide_tag_const :: "tag_const \<Rightarrow> tag_const \<Rightarrow> tag_const" where
+  fun divide_tag_const :: "'a tag_const \<Rightarrow> 'a tag_const \<Rightarrow> 'a tag_const" where
       Real_divide: "divide (Real n) (Real p) = (Real (divide n p))"
   instance proof qed
 end
 
-instantiation tag_const :: inverse
+instantiation tag_const :: (inverse)inverse
 begin
-  fun inverse_tag_const :: "tag_const \<Rightarrow> tag_const" where
+  fun inverse_tag_const :: "'a tag_const \<Rightarrow> 'a tag_const" where
       Real_inverse: "inverse (Real n) = (Real (inverse n))"
   instance proof qed
 end
 
-instantiation tag_const :: order
+instantiation tag_const :: (order)order
 begin
-  inductive less_eq_tag_const :: "tag_const \<Rightarrow> tag_const \<Rightarrow> bool" where
+  inductive less_eq_tag_const :: "'a tag_const \<Rightarrow> 'a tag_const \<Rightarrow> bool" where
     Int_less_eq[simp]:      "n \<le> m \<Longrightarrow> (Real n) \<le> (Real m)"
-  definition less_tag: "(x::tag_const) < y \<longleftrightarrow> (x \<le> y) \<and> (x \<noteq> y)"
+  definition less_tag: "(x::'a tag_const) < y \<longleftrightarrow> (x \<le> y) \<and> (x \<noteq> y)"
   instance proof
-    show "\<And>x y :: tag_const. (x < y) = (x \<le> y \<and> \<not> y \<le> x)"
+    show "\<And>x y :: 'a tag_const. (x < y) = (x \<le> y \<and> \<not> y \<le> x)"
       using less_eq_tag_const.simps less_tag by auto
-    show "\<And>x  :: tag_const. x \<le> x"
+    show "\<And>x  :: 'a tag_const. x \<le> x"
       by (metis (full_types) Int_less_eq order_refl tag_const.exhaust)
-    show "\<And>x y z  :: tag_const. x \<le> y \<Longrightarrow> y \<le> z \<Longrightarrow> x \<le> z"
+    show "\<And>x y z  :: 'a tag_const. x \<le> y \<Longrightarrow> y \<le> z \<Longrightarrow> x \<le> z"
       using less_eq_tag_const.simps by auto
-    show "\<And>x y  :: tag_const. x \<le> y \<Longrightarrow> y \<le> x \<Longrightarrow> x = y"
+    show "\<And>x y  :: 'a tag_const. x \<le> y \<Longrightarrow> y \<le> x \<Longrightarrow> x = y"
       using less_eq_tag_const.simps by auto
   qed
 end
 
-instantiation tag_const :: linorder
+instantiation tag_const :: (linorder)linorder
 begin
   instance proof
-    show "\<And>x y. (x::tag_const) \<le> y \<or> y \<le> x"
+    show "\<And>x y. (x::'a tag_const) \<le> y \<or> y \<le> x"
       by (metis (full_types) Int_less_eq le_cases tag_const.exhaust)
   qed
 end
