src/Denotational.thy
@@ -9,7 +9,7 @@ section \<open>Denotational interpretation for atomic TESL formulae\<close>
 
 (* Denotational interpretation of TESL atomic formulae *)
 fun TESL_interpretation_atomic
-    :: "TESL_atomic \<Rightarrow> run set" ("\<lbrakk> _ \<rbrakk>\<^sub>T\<^sub>E\<^sub>S\<^sub>L") where
+    :: "('\<tau>::linordered_field) TESL_atomic \<Rightarrow> '\<tau> run set" ("\<lbrakk> _ \<rbrakk>\<^sub>T\<^sub>E\<^sub>S\<^sub>L") where
     "\<lbrakk> K sporadic \<tau> \<rbrakk>\<^sub>T\<^sub>E\<^sub>S\<^sub>L =
         { \<rho>. \<exists>n::nat. hamlet ((Rep_run \<rho>) n K) = True \<and> time ((Rep_run \<rho>) n K) = \<tau> }"
   | "\<lbrakk> K\<^sub>1 sporadic \<lfloor>\<tau>\<rfloor> on K\<^sub>2 \<rbrakk>\<^sub>T\<^sub>E\<^sub>S\<^sub>L =
@@ -33,7 +33,7 @@ fun TESL_interpretation_atomic
 
 section \<open>Denotational interpretation for TESL formulae\<close>
 
-fun TESL_interpretation :: "TESL_formula \<Rightarrow> run set" ("\<lbrakk>\<lbrakk> _ \<rbrakk>\<rbrakk>\<^sub>T\<^sub>E\<^sub>S\<^sub>L") where
+fun TESL_interpretation :: "('\<tau>::linordered_field) TESL_formula \<Rightarrow> '\<tau> run set" ("\<lbrakk>\<lbrakk> _ \<rbrakk>\<rbrakk>\<^sub>T\<^sub>E\<^sub>S\<^sub>L") where
     "\<lbrakk>\<lbrakk> [] \<rbrakk>\<rbrakk>\<^sub>T\<^sub>E\<^sub>S\<^sub>L = { _. True }"
   | "\<lbrakk>\<lbrakk> \<phi> # \<Phi> \<rbrakk>\<rbrakk>\<^sub>T\<^sub>E\<^sub>S\<^sub>L = \<lbrakk> \<phi> \<rbrakk>\<^sub>T\<^sub>E\<^sub>S\<^sub>L \<inter> \<lbrakk>\<lbrakk> \<Phi> \<rbrakk>\<rbrakk>\<^sub>T\<^sub>E\<^sub>S\<^sub>L"
 
@@ -79,7 +79,7 @@ lemma TESL_interp_commute:
 
 lemma TESL_interp_left_commute:
   shows "\<lbrakk>\<lbrakk> \<Phi>\<^sub>1 @ (\<Phi>\<^sub>2 @ \<Phi>\<^sub>3) \<rbrakk>\<rbrakk>\<^sub>T\<^sub>E\<^sub>S\<^sub>L = \<lbrakk>\<lbrakk> \<Phi>\<^sub>2 @ (\<Phi>\<^sub>1 @ \<Phi>\<^sub>3) \<rbrakk>\<rbrakk>\<^sub>T\<^sub>E\<^sub>S\<^sub>L"
-  using TESL_interp_homo_append by auto
+  unfolding TESL_interp_homo_append by auto
 
 lemma TESL_interp_idem:
   shows "\<lbrakk>\<lbrakk> \<Phi> @ \<Phi> \<rbrakk>\<rbrakk>\<^sub>T\<^sub>E\<^sub>S\<^sub>L = \<lbrakk>\<lbrakk> \<Phi> \<rbrakk>\<rbrakk>\<^sub>T\<^sub>E\<^sub>S\<^sub>L"
@@ -91,7 +91,7 @@ lemma TESL_interp_left_idem:
 
 lemma TESL_interp_right_idem:
   shows "\<lbrakk>\<lbrakk> (\<Phi>\<^sub>1 @ \<Phi>\<^sub>2) @ \<Phi>\<^sub>2 \<rbrakk>\<rbrakk>\<^sub>T\<^sub>E\<^sub>S\<^sub>L = \<lbrakk>\<lbrakk> \<Phi>\<^sub>1 @ \<Phi>\<^sub>2 \<rbrakk>\<rbrakk>\<^sub>T\<^sub>E\<^sub>S\<^sub>L"
-  using TESL_interp_homo_append by auto
+  unfolding TESL_interp_homo_append by auto
 
 lemmas TESL_interp_aci = TESL_interp_commute TESL_interp_assoc TESL_interp_left_commute TESL_interp_left_idem
 
