src/Hygge_Theory.thy
@@ -45,7 +45,8 @@ lemma sound_reduction:
        (\<Gamma>\<^sub>2', n\<^sub>2' \<turnstile> \<Psi>\<^sub>2' \<triangleright> \<Phi>\<^sub>2') = (\<Gamma>, n \<turnstile> \<Psi> \<triangleright> (K sporadic \<tau>) # \<Phi>) \<Longrightarrow>
        \<lbrakk>\<lbrakk> \<Gamma>\<^sub>2 \<rbrakk>\<rbrakk>\<^sub>p\<^sub>r\<^sub>i\<^sub>m \<inter> \<lbrakk>\<lbrakk> \<Psi>\<^sub>2 \<rbrakk>\<rbrakk>\<^sub>T\<^sub>E\<^sub>S\<^sub>L\<^bsup>\<ge> n\<^sub>2\<^esup> \<inter> \<lbrakk>\<lbrakk> \<Phi>\<^sub>2 \<rbrakk>\<rbrakk>\<^sub>T\<^sub>E\<^sub>S\<^sub>L\<^bsup>\<ge> Suc n\<^sub>2\<^esup>
        \<subseteq> \<lbrakk>\<lbrakk> \<Gamma>\<^sub>1 \<rbrakk>\<rbrakk>\<^sub>p\<^sub>r\<^sub>i\<^sub>m \<inter> \<lbrakk>\<lbrakk> \<Psi>\<^sub>1 \<rbrakk>\<rbrakk>\<^sub>T\<^sub>E\<^sub>S\<^sub>L\<^bsup>\<ge> n\<^sub>1\<^esup> \<inter> \<lbrakk>\<lbrakk> \<Phi>\<^sub>1 \<rbrakk>\<rbrakk>\<^sub>T\<^sub>E\<^sub>S\<^sub>L\<^bsup>\<ge> Suc n\<^sub>1\<^esup>"
-      using HeronConf_interp_stepwise_sporadic_cases by auto
+      using HeronConf_interp_stepwise_sporadic_cases
+      by (metis HeronConf_interpretation.simps Un_upper1)
     show "\<And>\<Gamma>\<^sub>1' n\<^sub>1' \<Psi>\<^sub>1' \<Phi>\<^sub>1' \<Gamma>\<^sub>2' n\<^sub>2' \<Psi>\<^sub>2' \<Phi>\<^sub>2' \<Gamma> n K \<tau> \<Psi> \<Phi>.
        (\<Gamma>\<^sub>1, n\<^sub>1 \<turnstile> \<Psi>\<^sub>1 \<triangleright> \<Phi>\<^sub>1) = (\<Gamma>\<^sub>1', n\<^sub>1' \<turnstile> \<Psi>\<^sub>1' \<triangleright> \<Phi>\<^sub>1') \<Longrightarrow>
        (\<Gamma>\<^sub>2, n\<^sub>2 \<turnstile> \<Psi>\<^sub>2 \<triangleright> \<Phi>\<^sub>2) = (\<Gamma>\<^sub>2', n\<^sub>2' \<turnstile> \<Psi>\<^sub>2' \<triangleright> \<Phi>\<^sub>2') \<Longrightarrow>
@@ -61,7 +62,7 @@ lemma sound_reduction:
        (\<Gamma>\<^sub>2', n\<^sub>2' \<turnstile> \<Psi>\<^sub>2' \<triangleright> \<Phi>\<^sub>2') = (\<Gamma>, n \<turnstile> \<Psi> \<triangleright> (K\<^sub>1 sporadic \<tau> on K\<^sub>2) # \<Phi>) \<Longrightarrow>
        \<lbrakk>\<lbrakk> \<Gamma>\<^sub>2 \<rbrakk>\<rbrakk>\<^sub>p\<^sub>r\<^sub>i\<^sub>m \<inter> \<lbrakk>\<lbrakk> \<Psi>\<^sub>2 \<rbrakk>\<rbrakk>\<^sub>T\<^sub>E\<^sub>S\<^sub>L\<^bsup>\<ge> n\<^sub>2\<^esup> \<inter> \<lbrakk>\<lbrakk> \<Phi>\<^sub>2 \<rbrakk>\<rbrakk>\<^sub>T\<^sub>E\<^sub>S\<^sub>L\<^bsup>\<ge> Suc n\<^sub>2\<^esup>
        \<subseteq> \<lbrakk>\<lbrakk> \<Gamma>\<^sub>1 \<rbrakk>\<rbrakk>\<^sub>p\<^sub>r\<^sub>i\<^sub>m \<inter> \<lbrakk>\<lbrakk> \<Psi>\<^sub>1 \<rbrakk>\<rbrakk>\<^sub>T\<^sub>E\<^sub>S\<^sub>L\<^bsup>\<ge> n\<^sub>1\<^esup> \<inter> \<lbrakk>\<lbrakk> \<Phi>\<^sub>1 \<rbrakk>\<rbrakk>\<^sub>T\<^sub>E\<^sub>S\<^sub>L\<^bsup>\<ge> Suc n\<^sub>1\<^esup>"
-      using HeronConf_interp_stepwise_sporadicon_cases by auto
+      using HeronConf_interp_stepwise_sporadicon_cases by fastforce
     show "\<And>\<Gamma>\<^sub>1' n\<^sub>1' \<Psi>\<^sub>1' \<Phi>\<^sub>1' \<Gamma>\<^sub>2' n\<^sub>2' \<Psi>\<^sub>2' \<Phi>\<^sub>2' \<Gamma> n K\<^sub>1 \<tau> K\<^sub>2 \<Psi> \<Phi>.
        (\<Gamma>\<^sub>1, n\<^sub>1 \<turnstile> \<Psi>\<^sub>1 \<triangleright> \<Phi>\<^sub>1) = (\<Gamma>\<^sub>1', n\<^sub>1' \<turnstile> \<Psi>\<^sub>1' \<triangleright> \<Phi>\<^sub>1') \<Longrightarrow>
        (\<Gamma>\<^sub>2, n\<^sub>2 \<turnstile> \<Psi>\<^sub>2 \<triangleright> \<Phi>\<^sub>2) = (\<Gamma>\<^sub>2', n\<^sub>2' \<turnstile> \<Psi>\<^sub>2' \<triangleright> \<Phi>\<^sub>2') \<Longrightarrow>
@@ -69,7 +70,8 @@ lemma sound_reduction:
        (\<Gamma>\<^sub>2', n\<^sub>2' \<turnstile> \<Psi>\<^sub>2' \<triangleright> \<Phi>\<^sub>2') = (K\<^sub>1 \<Up> n # K\<^sub>2 \<Down> n @ \<tau> # \<Gamma>, n \<turnstile> \<Psi> \<triangleright> \<Phi>) \<Longrightarrow>
        \<lbrakk>\<lbrakk> \<Gamma>\<^sub>2 \<rbrakk>\<rbrakk>\<^sub>p\<^sub>r\<^sub>i\<^sub>m \<inter> \<lbrakk>\<lbrakk> \<Psi>\<^sub>2 \<rbrakk>\<rbrakk>\<^sub>T\<^sub>E\<^sub>S\<^sub>L\<^bsup>\<ge> n\<^sub>2\<^esup> \<inter> \<lbrakk>\<lbrakk> \<Phi>\<^sub>2 \<rbrakk>\<rbrakk>\<^sub>T\<^sub>E\<^sub>S\<^sub>L\<^bsup>\<ge> Suc n\<^sub>2\<^esup>
        \<subseteq> \<lbrakk>\<lbrakk> \<Gamma>\<^sub>1 \<rbrakk>\<rbrakk>\<^sub>p\<^sub>r\<^sub>i\<^sub>m \<inter> \<lbrakk>\<lbrakk> \<Psi>\<^sub>1 \<rbrakk>\<rbrakk>\<^sub>T\<^sub>E\<^sub>S\<^sub>L\<^bsup>\<ge> n\<^sub>1\<^esup> \<inter> \<lbrakk>\<lbrakk> \<Phi>\<^sub>1 \<rbrakk>\<rbrakk>\<^sub>T\<^sub>E\<^sub>S\<^sub>L\<^bsup>\<ge> Suc n\<^sub>1\<^esup>"
-      using HeronConf_interp_stepwise_sporadicon_cases by auto
+      using HeronConf_interp_stepwise_sporadicon_cases
+      by fastforce
     show "\<And>\<Gamma>\<^sub>1' n\<^sub>1' \<Psi>\<^sub>1' \<Phi>\<^sub>1' \<Gamma>\<^sub>2' n\<^sub>2' \<Psi>\<^sub>2' \<Phi>\<^sub>2' \<Gamma> n K\<^sub>1 \<alpha> K\<^sub>2 \<beta> \<Psi> \<Phi>.
        (\<Gamma>\<^sub>1, n\<^sub>1 \<turnstile> \<Psi>\<^sub>1 \<triangleright> \<Phi>\<^sub>1) = \<Gamma>\<^sub>1', n\<^sub>1' \<turnstile> \<Psi>\<^sub>1' \<triangleright> \<Phi>\<^sub>1' \<Longrightarrow>
        (\<Gamma>\<^sub>2, n\<^sub>2 \<turnstile> \<Psi>\<^sub>2 \<triangleright> \<Phi>\<^sub>2) = \<Gamma>\<^sub>2', n\<^sub>2' \<turnstile> \<Psi>\<^sub>2' \<triangleright> \<Phi>\<^sub>2' \<Longrightarrow>
@@ -79,7 +81,8 @@ lemma sound_reduction:
        \<Gamma>, n \<turnstile> \<Psi> \<triangleright> (tag-relation K\<^sub>1 = \<alpha> * K\<^sub>2 + \<beta>) # \<Phi> \<Longrightarrow>
        \<lbrakk>\<lbrakk> \<Gamma>\<^sub>2 \<rbrakk>\<rbrakk>\<^sub>p\<^sub>r\<^sub>i\<^sub>m \<inter> \<lbrakk>\<lbrakk> \<Psi>\<^sub>2 \<rbrakk>\<rbrakk>\<^sub>T\<^sub>E\<^sub>S\<^sub>L\<^bsup>\<ge> n\<^sub>2\<^esup> \<inter> \<lbrakk>\<lbrakk> \<Phi>\<^sub>2 \<rbrakk>\<rbrakk>\<^sub>T\<^sub>E\<^sub>S\<^sub>L\<^bsup>\<ge> Suc n\<^sub>2\<^esup>
        \<subseteq> \<lbrakk>\<lbrakk> \<Gamma>\<^sub>1 \<rbrakk>\<rbrakk>\<^sub>p\<^sub>r\<^sub>i\<^sub>m \<inter> \<lbrakk>\<lbrakk> \<Psi>\<^sub>1 \<rbrakk>\<rbrakk>\<^sub>T\<^sub>E\<^sub>S\<^sub>L\<^bsup>\<ge> n\<^sub>1\<^esup> \<inter> \<lbrakk>\<lbrakk> \<Phi>\<^sub>1 \<rbrakk>\<rbrakk>\<^sub>T\<^sub>E\<^sub>S\<^sub>L\<^bsup>\<ge> Suc n\<^sub>1\<^esup>"
-      using HeronConf_interp_stepwise_tagrel_cases by auto
+      using HeronConf_interp_stepwise_tagrel_cases
+      by (metis HeronConf_interpretation.simps equalityD1)
     show "\<And>\<Gamma>\<^sub>1' n\<^sub>1' \<Psi>\<^sub>1' \<Phi>\<^sub>1' \<Gamma>\<^sub>2' n\<^sub>2' \<Psi>\<^sub>2' \<Phi>\<^sub>2' \<Gamma> n K\<^sub>1 K\<^sub>2 R \<Psi> \<Phi>.
        (\<Gamma>\<^sub>1, n\<^sub>1 \<turnstile> \<Psi>\<^sub>1 \<triangleright> \<Phi>\<^sub>1) = \<Gamma>\<^sub>1', n\<^sub>1' \<turnstile> \<Psi>\<^sub>1' \<triangleright> \<Phi>\<^sub>1' \<Longrightarrow>
        (\<Gamma>\<^sub>2, n\<^sub>2 \<turnstile> \<Psi>\<^sub>2 \<triangleright> \<Phi>\<^sub>2) = \<Gamma>\<^sub>2', n\<^sub>2' \<turnstile> \<Psi>\<^sub>2' \<triangleright> \<Phi>\<^sub>2' \<Longrightarrow>
@@ -87,7 +90,8 @@ lemma sound_reduction:
        (\<Gamma>\<^sub>2', n\<^sub>2' \<turnstile> \<Psi>\<^sub>2' \<triangleright> \<Phi>\<^sub>2') = \<langle>\<tau>\<^sub>v\<^sub>a\<^sub>r(K\<^sub>1, n), \<tau>\<^sub>v\<^sub>a\<^sub>r(K\<^sub>2, n)\<rangle> \<epsilon> R # \<Gamma>, n \<turnstile> \<Psi> \<triangleright> (tag-relation \<langle>K\<^sub>1, K\<^sub>2\<rangle> \<in> R) # \<Phi> \<Longrightarrow>
        \<lbrakk>\<lbrakk> \<Gamma>\<^sub>2 \<rbrakk>\<rbrakk>\<^sub>p\<^sub>r\<^sub>i\<^sub>m \<inter> \<lbrakk>\<lbrakk> \<Psi>\<^sub>2 \<rbrakk>\<rbrakk>\<^sub>T\<^sub>E\<^sub>S\<^sub>L\<^bsup>\<ge> n\<^sub>2\<^esup> \<inter> \<lbrakk>\<lbrakk> \<Phi>\<^sub>2 \<rbrakk>\<rbrakk>\<^sub>T\<^sub>E\<^sub>S\<^sub>L\<^bsup>\<ge> Suc n\<^sub>2\<^esup>
        \<subseteq> \<lbrakk>\<lbrakk> \<Gamma>\<^sub>1 \<rbrakk>\<rbrakk>\<^sub>p\<^sub>r\<^sub>i\<^sub>m \<inter> \<lbrakk>\<lbrakk> \<Psi>\<^sub>1 \<rbrakk>\<rbrakk>\<^sub>T\<^sub>E\<^sub>S\<^sub>L\<^bsup>\<ge> n\<^sub>1\<^esup> \<inter> \<lbrakk>\<lbrakk> \<Phi>\<^sub>1 \<rbrakk>\<rbrakk>\<^sub>T\<^sub>E\<^sub>S\<^sub>L\<^bsup>\<ge> Suc n\<^sub>1\<^esup>"
-      using HeronConf_interp_stepwise_tagrelgen_cases by auto
+      using HeronConf_interp_stepwise_tagrelgen_cases
+      by (metis HeronConf_interpretation.simps equalityD1)
     show "\<And>\<Gamma>\<^sub>1' n\<^sub>1' \<Psi>\<^sub>1' \<Phi>\<^sub>1' \<Gamma>\<^sub>2' n\<^sub>2' \<Psi>\<^sub>2' \<Phi>\<^sub>2' \<Gamma> n K\<^sub>1 K\<^sub>2 \<Psi> \<Phi>.
        (\<Gamma>\<^sub>1, n\<^sub>1 \<turnstile> \<Psi>\<^sub>1 \<triangleright> \<Phi>\<^sub>1) = \<Gamma>\<^sub>1', n\<^sub>1' \<turnstile> \<Psi>\<^sub>1' \<triangleright> \<Phi>\<^sub>1' \<Longrightarrow>
        (\<Gamma>\<^sub>2, n\<^sub>2 \<turnstile> \<Psi>\<^sub>2 \<triangleright> \<Phi>\<^sub>2) = \<Gamma>\<^sub>2', n\<^sub>2' \<turnstile> \<Psi>\<^sub>2' \<triangleright> \<Phi>\<^sub>2' \<Longrightarrow>
@@ -95,7 +99,8 @@ lemma sound_reduction:
        (\<Gamma>\<^sub>2', n\<^sub>2' \<turnstile> \<Psi>\<^sub>2' \<triangleright> \<Phi>\<^sub>2') = K\<^sub>1 \<not>\<Up> n # \<Gamma>, n \<turnstile> \<Psi> \<triangleright> (K\<^sub>1 implies K\<^sub>2) # \<Phi> \<Longrightarrow>
        \<lbrakk>\<lbrakk> \<Gamma>\<^sub>2 \<rbrakk>\<rbrakk>\<^sub>p\<^sub>r\<^sub>i\<^sub>m \<inter> \<lbrakk>\<lbrakk> \<Psi>\<^sub>2 \<rbrakk>\<rbrakk>\<^sub>T\<^sub>E\<^sub>S\<^sub>L\<^bsup>\<ge> n\<^sub>2\<^esup> \<inter> \<lbrakk>\<lbrakk> \<Phi>\<^sub>2 \<rbrakk>\<rbrakk>\<^sub>T\<^sub>E\<^sub>S\<^sub>L\<^bsup>\<ge> Suc n\<^sub>2\<^esup>
        \<subseteq> \<lbrakk>\<lbrakk> \<Gamma>\<^sub>1 \<rbrakk>\<rbrakk>\<^sub>p\<^sub>r\<^sub>i\<^sub>m \<inter> \<lbrakk>\<lbrakk> \<Psi>\<^sub>1 \<rbrakk>\<rbrakk>\<^sub>T\<^sub>E\<^sub>S\<^sub>L\<^bsup>\<ge> n\<^sub>1\<^esup> \<inter> \<lbrakk>\<lbrakk> \<Phi>\<^sub>1 \<rbrakk>\<rbrakk>\<^sub>T\<^sub>E\<^sub>S\<^sub>L\<^bsup>\<ge> Suc n\<^sub>1\<^esup>"
-      using HeronConf_interp_stepwise_implies_cases by auto
+      using HeronConf_interp_stepwise_implies_cases
+      by (metis HeronConf_interpretation.simps inf_sup_ord(3))
     show "\<And>\<Gamma>\<^sub>1' n\<^sub>1' \<Psi>\<^sub>1' \<Phi>\<^sub>1' \<Gamma>\<^sub>2' n\<^sub>2' \<Psi>\<^sub>2' \<Phi>\<^sub>2' \<Gamma> n K\<^sub>1 K\<^sub>2 \<Psi> \<Phi>.
        (\<Gamma>\<^sub>1, n\<^sub>1 \<turnstile> \<Psi>\<^sub>1 \<triangleright> \<Phi>\<^sub>1) = (\<Gamma>\<^sub>1', n\<^sub>1' \<turnstile> \<Psi>\<^sub>1' \<triangleright> \<Phi>\<^sub>1') \<Longrightarrow>
        (\<Gamma>\<^sub>2, n\<^sub>2 \<turnstile> \<Psi>\<^sub>2 \<triangleright> \<Phi>\<^sub>2) = (\<Gamma>\<^sub>2', n\<^sub>2' \<turnstile> \<Psi>\<^sub>2' \<triangleright> \<Phi>\<^sub>2') \<Longrightarrow>
@@ -103,7 +108,8 @@ lemma sound_reduction:
        (\<Gamma>\<^sub>2', n\<^sub>2' \<turnstile> \<Psi>\<^sub>2' \<triangleright> \<Phi>\<^sub>2') = (K\<^sub>1 \<Up> n # K\<^sub>2 \<Up> n # \<Gamma>, n \<turnstile> \<Psi> \<triangleright> (K\<^sub>1 implies K\<^sub>2) # \<Phi>) \<Longrightarrow>
        \<lbrakk>\<lbrakk> \<Gamma>\<^sub>2 \<rbrakk>\<rbrakk>\<^sub>p\<^sub>r\<^sub>i\<^sub>m \<inter> \<lbrakk>\<lbrakk> \<Psi>\<^sub>2 \<rbrakk>\<rbrakk>\<^sub>T\<^sub>E\<^sub>S\<^sub>L\<^bsup>\<ge> n\<^sub>2\<^esup> \<inter> \<lbrakk>\<lbrakk> \<Phi>\<^sub>2 \<rbrakk>\<rbrakk>\<^sub>T\<^sub>E\<^sub>S\<^sub>L\<^bsup>\<ge> Suc n\<^sub>2\<^esup>
        \<subseteq> \<lbrakk>\<lbrakk> \<Gamma>\<^sub>1 \<rbrakk>\<rbrakk>\<^sub>p\<^sub>r\<^sub>i\<^sub>m \<inter> \<lbrakk>\<lbrakk> \<Psi>\<^sub>1 \<rbrakk>\<rbrakk>\<^sub>T\<^sub>E\<^sub>S\<^sub>L\<^bsup>\<ge> n\<^sub>1\<^esup> \<inter> \<lbrakk>\<lbrakk> \<Phi>\<^sub>1 \<rbrakk>\<rbrakk>\<^sub>T\<^sub>E\<^sub>S\<^sub>L\<^bsup>\<ge> Suc n\<^sub>1\<^esup>"
-      using HeronConf_interp_stepwise_implies_cases by auto
+      using HeronConf_interp_stepwise_implies_cases
+      by (metis HeronConf_interpretation.simps inf_sup_ord(4))
     show "\<And>\<Gamma>\<^sub>1' n\<^sub>1' \<Psi>\<^sub>1' \<Phi>\<^sub>1' \<Gamma>\<^sub>2' n\<^sub>2' \<Psi>\<^sub>2' \<Phi>\<^sub>2' \<Gamma> n K\<^sub>1 \<delta>\<tau> K\<^sub>2 K\<^sub>3 \<Psi> \<Phi>.
        (\<Gamma>\<^sub>1, n\<^sub>1 \<turnstile> \<Psi>\<^sub>1 \<triangleright> \<Phi>\<^sub>1) = (\<Gamma>\<^sub>1', n\<^sub>1' \<turnstile> \<Psi>\<^sub>1' \<triangleright> \<Phi>\<^sub>1') \<Longrightarrow>
        (\<Gamma>\<^sub>2, n\<^sub>2 \<turnstile> \<Psi>\<^sub>2 \<triangleright> \<Phi>\<^sub>2) = (\<Gamma>\<^sub>2', n\<^sub>2' \<turnstile> \<Psi>\<^sub>2' \<triangleright> \<Phi>\<^sub>2') \<Longrightarrow>
@@ -112,7 +118,8 @@ lemma sound_reduction:
        K\<^sub>1 \<not>\<Up> n # \<Gamma>, n \<turnstile> \<Psi> \<triangleright> (K\<^sub>1 time-delayed by \<delta>\<tau> on K\<^sub>2 implies K\<^sub>3) # \<Phi> \<Longrightarrow>
        \<lbrakk>\<lbrakk> \<Gamma>\<^sub>2 \<rbrakk>\<rbrakk>\<^sub>p\<^sub>r\<^sub>i\<^sub>m \<inter> \<lbrakk>\<lbrakk> \<Psi>\<^sub>2 \<rbrakk>\<rbrakk>\<^sub>T\<^sub>E\<^sub>S\<^sub>L\<^bsup>\<ge> n\<^sub>2\<^esup> \<inter> \<lbrakk>\<lbrakk> \<Phi>\<^sub>2 \<rbrakk>\<rbrakk>\<^sub>T\<^sub>E\<^sub>S\<^sub>L\<^bsup>\<ge> Suc n\<^sub>2\<^esup>
        \<subseteq> \<lbrakk>\<lbrakk> \<Gamma>\<^sub>1 \<rbrakk>\<rbrakk>\<^sub>p\<^sub>r\<^sub>i\<^sub>m \<inter> \<lbrakk>\<lbrakk> \<Psi>\<^sub>1 \<rbrakk>\<rbrakk>\<^sub>T\<^sub>E\<^sub>S\<^sub>L\<^bsup>\<ge> n\<^sub>1\<^esup> \<inter> \<lbrakk>\<lbrakk> \<Phi>\<^sub>1 \<rbrakk>\<rbrakk>\<^sub>T\<^sub>E\<^sub>S\<^sub>L\<^bsup>\<ge> Suc n\<^sub>1\<^esup>"
-      using HeronConf_interp_stepwise_timedelayed_cases by auto
+      using HeronConf_interp_stepwise_timedelayed_cases
+      by (metis (no_types, lifting) HeronConf_interpretation.simps inf.order_iff inf_sup_absorb)
     show "\<And>\<Gamma>\<^sub>1' n\<^sub>1' \<Psi>\<^sub>1' \<Phi>\<^sub>1' \<Gamma>\<^sub>2' n\<^sub>2' \<Psi>\<^sub>2' \<Phi>\<^sub>2' \<Gamma> n K\<^sub>1 \<delta>\<tau> K\<^sub>2 K\<^sub>3 \<Psi> \<Phi>.
        (\<Gamma>\<^sub>1, n\<^sub>1 \<turnstile> \<Psi>\<^sub>1 \<triangleright> \<Phi>\<^sub>1) = (\<Gamma>\<^sub>1', n\<^sub>1' \<turnstile> \<Psi>\<^sub>1' \<triangleright> \<Phi>\<^sub>1') \<Longrightarrow>
        (\<Gamma>\<^sub>2, n\<^sub>2 \<turnstile> \<Psi>\<^sub>2 \<triangleright> \<Phi>\<^sub>2) = (\<Gamma>\<^sub>2', n\<^sub>2' \<turnstile> \<Psi>\<^sub>2' \<triangleright> \<Phi>\<^sub>2') \<Longrightarrow>
@@ -123,7 +130,8 @@ lemma sound_reduction:
                \<Psi> \<triangleright> (K\<^sub>1 time-delayed by \<delta>\<tau> on K\<^sub>2 implies K\<^sub>3) # \<Phi> \<Longrightarrow>
        \<lbrakk>\<lbrakk> \<Gamma>\<^sub>2 \<rbrakk>\<rbrakk>\<^sub>p\<^sub>r\<^sub>i\<^sub>m \<inter> \<lbrakk>\<lbrakk> \<Psi>\<^sub>2 \<rbrakk>\<rbrakk>\<^sub>T\<^sub>E\<^sub>S\<^sub>L\<^bsup>\<ge> n\<^sub>2\<^esup> \<inter> \<lbrakk>\<lbrakk> \<Phi>\<^sub>2 \<rbrakk>\<rbrakk>\<^sub>T\<^sub>E\<^sub>S\<^sub>L\<^bsup>\<ge> Suc n\<^sub>2\<^esup>
        \<subseteq> \<lbrakk>\<lbrakk> \<Gamma>\<^sub>1 \<rbrakk>\<rbrakk>\<^sub>p\<^sub>r\<^sub>i\<^sub>m \<inter> \<lbrakk>\<lbrakk> \<Psi>\<^sub>1 \<rbrakk>\<rbrakk>\<^sub>T\<^sub>E\<^sub>S\<^sub>L\<^bsup>\<ge> n\<^sub>1\<^esup> \<inter> \<lbrakk>\<lbrakk> \<Phi>\<^sub>1 \<rbrakk>\<rbrakk>\<^sub>T\<^sub>E\<^sub>S\<^sub>L\<^bsup>\<ge> Suc n\<^sub>1\<^esup>"
-      using HeronConf_interp_stepwise_timedelayed_cases by auto
+      using HeronConf_interp_stepwise_timedelayed_cases
+      by (metis HeronConf_interpretation.simps sup_ge2)
     qed
   qed
 
@@ -254,7 +262,8 @@ lemma instant_index_increase:
     then show ?case
       proof -
         have "\<Gamma>, n \<turnstile> [] \<triangleright> \<Phi> \<hookrightarrow>\<^bsup>1\<^esup> \<Gamma>, Suc n \<turnstile> \<Phi> \<triangleright> []"
-          using instant_i intro_part by auto
+          using instant_i intro_part
+          by fastforce
         moreover have "\<lbrakk> \<Gamma>, n \<turnstile> [] \<triangleright> \<Phi> \<rbrakk>\<^sub>c\<^sub>o\<^sub>n\<^sub>f\<^sub>i\<^sub>g = \<lbrakk> \<Gamma>, Suc n \<turnstile> \<Phi> \<triangleright> [] \<rbrakk>\<^sub>c\<^sub>o\<^sub>n\<^sub>f\<^sub>i\<^sub>g"
           by auto
         moreover have "\<rho> \<in> \<lbrakk> \<Gamma>, Suc n \<turnstile> \<Phi> \<triangleright> [] \<rbrakk>\<^sub>c\<^sub>o\<^sub>n\<^sub>f\<^sub>i\<^sub>g"
@@ -469,13 +478,13 @@ theorem progress:
 
 section \<open>Local termination\<close>
 
-primrec measure_interpretation :: "TESL_formula \<Rightarrow> nat" ("\<mu>") where
+primrec measure_interpretation :: "'\<tau> :: linordered_field TESL_formula \<Rightarrow> nat" ("\<mu>") where
     "\<mu> [] = (0::nat)"
   | "\<mu> (\<phi> # \<Phi>) = (case \<phi> of
                         _ sporadic _ on _ \<Rightarrow> 1 + \<mu> \<Phi>
                       | _                 \<Rightarrow> 2 + \<mu> \<Phi>)"
 
-fun measure_interpretation_config :: "config \<Rightarrow> nat" ("\<mu>\<^sub>c\<^sub>o\<^sub>n\<^sub>f\<^sub>i\<^sub>g") where
+fun measure_interpretation_config :: "'\<tau> :: linordered_field config \<Rightarrow> nat" ("\<mu>\<^sub>c\<^sub>o\<^sub>n\<^sub>f\<^sub>i\<^sub>g") where
     "\<mu>\<^sub>c\<^sub>o\<^sub>n\<^sub>f\<^sub>i\<^sub>g (\<Gamma>, n \<turnstile> \<Psi> \<triangleright> \<Phi>) = \<mu> \<Psi>"
 
 lemma elimation_rules_strictly_decreasing:
@@ -496,15 +505,15 @@ lemma elimation_rules_strictly_decreasing_meas':
 
 text \<open>The relation made up of elimination rules is well-founded.\<close>
 theorem instant_computation_termination:
-  shows "wfP (\<lambda>\<S>\<^sub>1 \<S>\<^sub>2. \<S>\<^sub>1  \<hookrightarrow>\<^sub>e\<^sup>\<leftarrow>  \<S>\<^sub>2)"
+  shows "wfP (\<lambda>(\<S>\<^sub>1:: 'a :: linordered_field config) \<S>\<^sub>2. \<S>\<^sub>1  \<hookrightarrow>\<^sub>e\<^sup>\<leftarrow>  \<S>\<^sub>2)"
   proof (simp add: wfP_def)
-    show "wf {(\<S>\<^sub>1, \<S>\<^sub>2). \<S>\<^sub>1 \<hookrightarrow>\<^sub>e\<^sup>\<leftarrow> \<S>\<^sub>2}"
+    show "wf {((\<S>\<^sub>1:: 'a :: linordered_field config), \<S>\<^sub>2). \<S>\<^sub>1 \<hookrightarrow>\<^sub>e\<^sup>\<leftarrow> \<S>\<^sub>2}"
     apply (rule wf_subset)
     proof -
-      have "measure \<mu>\<^sub>c\<^sub>o\<^sub>n\<^sub>f\<^sub>i\<^sub>g = { (\<S>\<^sub>2, \<S>\<^sub>1). \<mu>\<^sub>c\<^sub>o\<^sub>n\<^sub>f\<^sub>i\<^sub>g \<S>\<^sub>2 < \<mu>\<^sub>c\<^sub>o\<^sub>n\<^sub>f\<^sub>i\<^sub>g \<S>\<^sub>1 }"
+      have "measure \<mu>\<^sub>c\<^sub>o\<^sub>n\<^sub>f\<^sub>i\<^sub>g = { (\<S>\<^sub>2, (\<S>\<^sub>1:: 'a :: linordered_field config)). \<mu>\<^sub>c\<^sub>o\<^sub>n\<^sub>f\<^sub>i\<^sub>g \<S>\<^sub>2 < \<mu>\<^sub>c\<^sub>o\<^sub>n\<^sub>f\<^sub>i\<^sub>g \<S>\<^sub>1 }"
         by (simp add: inv_image_def less_eq measure_def)
-      then show "{(\<S>\<^sub>1, \<S>\<^sub>2). \<S>\<^sub>1 \<hookrightarrow>\<^sub>e\<^sup>\<leftarrow> \<S>\<^sub>2} \<subseteq> (measure \<mu>\<^sub>c\<^sub>o\<^sub>n\<^sub>f\<^sub>i\<^sub>g)"
-        using elimation_rules_strictly_decreasing_meas' operational_semantics_elim_inv_def by auto
+      then show "{((\<S>\<^sub>1:: 'a :: linordered_field config), \<S>\<^sub>2). \<S>\<^sub>1 \<hookrightarrow>\<^sub>e\<^sup>\<leftarrow> \<S>\<^sub>2} \<subseteq> (measure \<mu>\<^sub>c\<^sub>o\<^sub>n\<^sub>f\<^sub>i\<^sub>g)"
+        using elimation_rules_strictly_decreasing_meas' operational_semantics_elim_inv_def by blast
       show "wf (measure measure_interpretation_config)"
         by simp
     qed
